DeBruijnSSA/BinSyntax/Rewrite/Region/Setoid.lean
@@ -610,8 +610,8 @@ theorem InS.codiagonal {Γ : Ctx α ε} {L : LCtx α}
   sorry
 
 theorem InS.dinaturality {Γ : Ctx α ε} {R R' L : LCtx α}
-  {σ : Subst.InS φ Γ R R'} {β : InS φ Γ (R ++ L)}
+  {σ : Subst.InS φ Γ R (R' ++ L)} {β : InS φ Γ (R ++ L)}
   {G : (i : Fin R'.length) → InS φ (⟨R'.get i, ⊥⟩::Γ) (R ++ L)}
-  : cfg R' (β.lsubst σ.extend) (λi => (G i).lsubst σ.extend.vlift)
-  = cfg R β (λi => (σ.cfg i).lsubst (CFG.toSubst G).vlift)
+  : cfg R' (β.lsubst σ.extend_in) (λi => (G i).lsubst σ.extend_in.vlift)
+  = cfg R β (λi => (σ.cfg i).lsubst (CFG.toSubst_append G).vlift)
   := sorry
